code/experimental/ed25519/Hacl.Bignum25519.fsti
@@ -1,0 +1,69 @@
+module Hacl.Bignum25519
+
+#set-options "--lax"
+
+val red_513: Hacl.Bignum.Parameters.seqelem -> GTot Type0
+val red_53: Hacl.Bignum.Parameters.seqelem -> GTot Type0
+val red_5413: Hacl.Bignum.Parameters.seqelem -> GTot Type0
+
+(* abstract let red_513 s = Hacl.Spec.EC.AddAndDouble.red_513 s *)
+(* abstract let red_53 s = Hacl.Spec.EC.AddAndDouble.red_53 s *)
+(* abstract let red_5413 s = Hacl.Spec.EC.AddAndDouble.red_5413 s *)
+
+let felem = Hacl.Bignum.Parameters.felem
+
+val fsum:
+  a:felem ->
+  b:felem ->
+  St unit
+
+val fdifference:
+  a:felem ->
+  b:felem ->
+  St unit
+
+val reduce_513:
+  a:felem -> 
+  St unit
+
+val fdifference_reduced:
+  a:felem -> 
+  b:felem -> 
+  St unit
+
+val fmul:
+  out:felem ->
+  a:felem ->
+  b:felem ->
+  St unit
+
+val times_2:
+  out:felem ->
+  a:felem ->
+  St unit
+
+val times_d:
+  out:felem ->
+  a:felem ->
+  St unit
+
+val times_2d:
+  out:felem ->
+  a:felem ->
+  St unit
+
+val fsquare:
+  out:felem ->
+  a:felem ->
+  St unit
+
+val fsquare_times:
+  out:felem ->
+  a:felem ->
+  n:UInt32.t ->
+  St unit
+
+val inverse:
+  out:felem ->
+  a:felem ->
+  St unit
