code/experimental/ed25519/Hacl.Impl.Ed25519.RecoverX.fst
@@ -1,0 +1,26 @@
+module Hacl.Impl.Ed25519.RecoverX
+
+open FStar.Buffer
+open Hacl.Spec.BignumQ.Eval
+
+let qelemB = b:buffer Hacl.UInt64.t{length b = 5}
+
+val recover_x:
+  x:qelemB ->
+  y:qelemB{disjoint x y} ->
+  sign:Hacl.UInt64.t ->
+  Stack FStar.UInt32.t
+    (requires (fun h -> live h x /\ live h y))
+    (ensures (fun h0 _ h1 -> live h1 x /\ live h0 y /\ modifies_1 x h0 h1))
+let recover_x x y sign =
+  push_frame();
+  let m = create 0uL 5ul in
+  let m = Hacl.Impl.BignumQ.Mul.make_m m in
+  Hacl.Impl.BignumQ.Mul.subm_conditional x y m;
+  let x4 = x.(4ul) in
+  let res =
+  if FStar.UInt64 (x4 >= 0x10000000000uL) then 1uL
+  else (
+    // Compute ((y `fmul` y) `fsub` 1) `fmul` (modp_inv ((d `fmul` y `fmul` y) `fadd` one))
+    
+  )
