code/experimental/ed25519/Hacl.Impl.Ed25519.Sign.fst
@@ -1,0 +1,4 @@
+module Hacl.Impl.Ed25519.Sign
+
+open FStar.Buffer
+
