code/experimental/ed25519/Hacl.Impl.SHA512.ModQ.fst
@@ -1,0 +1,23 @@
+module Hacl.Impl.SHA512.ModQ
+
+open FStar.Buffer
+open Hacl.Impl.BignumQ.Mul
+
+val sha512_modq:
+  out:qelemB ->
+  input:buffer Hacl.UInt8.t ->
+  len  :UInt32.t{UInt32.v len = length input} ->
+  Stack unit
+        (requires (fun h0 -> live h0 input /\ live h0 out))
+        (ensures  (fun h0 _ h1 -> live h0 input /\ live h1 out /\ modifies_1 out h0 h1 /\
+          Hacl.Spec.BignumQ.Eval.eval_q (as_seq h1 out) == Spec.Ed25519.sha512_modq (as_seq h0 input)))
+let sha512_modq out input len =
+  push_frame();
+  let tmp = create (Hacl.Cast.uint64_to_sint64 0uL) 10ul in
+  push_frame();
+  let hash = create (Hacl.Cast.uint8_to_sint8 0uy) 64ul in
+  Hacl.Impl.Sha512.sha512 hash input len;
+  Hacl.Impl.Load56.load_64_bytes tmp hash;
+  pop_frame();
+  Hacl.Impl.BignumQ.Mul.barrett_reduction out tmp;
+  pop_frame()
