code/experimental/ed25519/Hacl.Impl.Sha512.fst
@@ -1,0 +1,12 @@
+module Hacl.Impl.Sha512
+
+open FStar.Buffer
+
+assume val sha512:
+  hash :buffer Hacl.UInt8.t{length hash = 64} ->
+  input:buffer Hacl.UInt8.t ->
+  len  :UInt32.t{UInt32.v len = length input} ->
+  Stack unit
+        (requires (fun h0 -> live h0 hash /\ live h0 input))
+        (ensures  (fun h0 _ h1 -> live h0 input /\ live h1 hash /\ modifies_1 hash h0 h1 /\
+                  as_seq h1 hash == Spec.Sha512.sha512 (as_seq h0 input)))
